packet definitions

LiveVerif/src/LiveVerifExamples/mbuf.v
@@ -3,7 +3,12 @@ Require Import LiveVerif.LiveVerifLib.
 
 Load LiveVerif.
 
-Definition MBUF_SIZE := 2048.
+Notation ".* */ '#define' lhs rhs /* *" := (lhs = rhs)
+  (at level 200, lhs constr at level 0, rhs constr at level 0, only parsing).
+
+Definition MBUF_SIZE := 2048. Remark MBUF_SIZE_def: .**/
+#define MBUF_SIZE 2048
+/**. reflexivity. Qed.
 
 (* Note: this will result in mbufs slightly bigger than half of a 4KB page,
    so most mbufs will span two pages, which seems bad --> don't do this!
@@ -18,9 +23,45 @@ Definition mbuf(r: mbuf_t): word -> mem -> Prop := .**/
   } mbuf;
 /**. *)
 
+(* Note: this is not easily compatible with viewing a buffer as a more structured packet
 Definition mbuf(n: Z)(bs: list Z)(a: word): mem -> Prop :=
   <{ * array (uint 8) n bs a
-     * array (uint 8) (MBUF_SIZE - n) ? (a ^+ /[n]) }>.
+     * array (uint 8) (MBUF_SIZE - n) ? (a ^+ /[n]) }>. *)
+
+(* Note: this is not easily compatible with predicates that combine headers & payload
+   (to put length of payload into headers)
+Definition mbuf
+  (headers: word -> mem -> Prop){headers_sz: PredicateSize headers}
+  (payload: word -> mem -> Prop){payload_sz: PredicateSize payload}
+  : word -> mem -> Prop :=
+  <{ + headers
+     + payload
+     + anyval (array (uint 8) (MBUF_SIZE - headers_sz - payload_sz)) }>. *)
+
+(* Note: requiring a packet_sz for a potentially abstract packet predicate
+   is a bit awkward, because quantifying over {packet_sz: PredicateSize packet}
+   in a function spec will put it into a forall, where we can't really mark
+   arguments as implicit, and we will typically still pass the size as a
+   non-ghost parameter, so we need an equality between the ghost size and the
+   actual size, all a bit awkward
+Definition mbuf(packet: word -> mem -> Prop){packet_sz: PredicateSize packet}
+  : word -> mem -> Prop :=
+  <{ + packet
+     + anyval (array (uint 8) (MBUF_SIZE - packet_sz)) }>.
+
+So we just make the packet_sz argument explicit:
+
+Definition mbuf(packet: word -> mem -> Prop)(packet_sz: PredicateSize packet)
+  : word -> mem -> Prop :=
+  <{ + packet
+     + anyval (array (uint 8) (MBUF_SIZE - packet_sz)) }>.
+
+But now, putting the size after the packet is a bit awkward (because eg in array,
+size comes first. *)
+
+Definition mbuf(packet_sz: Z)(packet: word -> mem -> Prop)(addr: word): mem -> Prop :=
+  <{ * packet addr
+     * array (uint 8) (MBUF_SIZE - packet_sz) ? (addr ^+ /[packet_sz]) }>.
 
 End LiveVerif.
 
