LiveVerif/src/LiveVerifExamples/network.v
@@ -4,15 +4,14 @@ Require Import bedrock2.TraceInspection.
 Require Import bedrock2.NetworkPackets.
 Require Import bedrock2.e1000_packet_trace.
 Require Import LiveVerifExamples.mbuf.
-Require Import LiveVerifExamples.e1000.
 
-Record headers_upto_ip: Set := {
+Record headers_upto_ip_t: Set := {
   before_ip_header: ethernet_header_t;
   only_ip_header: ip_header_t;
 }.
 
-Record headers_upto_udp: Set := {
-  before_udp_header: headers_upto_ip;
+Record headers_upto_udp_t: Set := {
+  before_udp_header: headers_upto_ip_t;
   only_udp_header: udp_header_t;
 }.
 
@@ -20,50 +19,15 @@ Require Import coqutil.Map.OfListWord.
 
 Load LiveVerif.
 
+Definition headers_upto_ip(h: headers_upto_ip_t): word -> mem -> Prop :=
+  <{ + ethernet_header (before_ip_header h)
+     + ip_header (only_ip_header h) }>.
+
+Definition headers_upto_udp(h: headers_upto_udp_t): word -> mem -> Prop :=
+  <{ + headers_upto_ip (before_udp_header h)
+     + udp_header (only_udp_header h) }>.
 
 (* in the packet_trace, the excess bytes of mbufs don't appear, but in mbufs, they do *)
-
-(*
-Definition mbuf(payload: list byte -> Prop): list byte -> Prop :=
-  and_preds (has_len MBUF_SIZE) (concat_preds payload any).
-
-(*
-Definition mbuf(n: Z)(bs: list Z): list byte -> Prop :=
-  and_preds (has_len MBUF_SIZE) (concat_preds (and_preds (has_len n) (eqZs bs)) any).
-*)
-
-Definition eth_header_bytes(h: ethernet_header_t): list byte -> Prop. Admitted.
-Definition ip_header_bytes(h: ip_header_t): list byte -> Prop. Admitted.
-Definition udp_header_bytes(h: udp_header_t): list byte -> Prop. Admitted.
-
-Definition eth_buf(h: ethernet_header_t)(payload: list byte -> Prop): list byte -> Prop :=
-  mbuf (concat_preds (eth_header_bytes h) payload).
-
-Definition ip_buf(eh: ethernet_header_t)(ih: ip_header_t)
-  (payload: list byte -> Prop): list byte -> Prop :=
-  eth_buf eh (concat_preds (ip_header_bytes ih) payload).
-
-Definition udp_buf(eh: ethernet_header_t)(ih: ip_header_t)(uh: udp_header_t)
-  (payload: list byte -> Prop): list byte -> Prop :=
-  ip_buf eh ih (concat_preds (udp_header_bytes uh) payload).
-*)
-
-(*
-Definition eth_buf(h: ethernet_header_t)(n: Z)(bs: list Z): word -> mem -> Prop :=
-  exists header_bytes, decode_ethernet_header header_bytes = h /\
-  mbuf (sizeof ethernet_header + n) (header_bytes ++ bs)
-
-  <{ * ethernet_header h a
-     * array (uint 8) n bs (a ^+ /[sizeof ethernet_header])
-     * array (uint 8) (MBUF_SIZE - n - sizeof ethernet_header) ?
-         (a ^+ /[sizeof ethernet_header + n]) }>.
-
-Definition eth_buf(h: ethernet_header_t)(n: Z)(bs: list Z)(a: word): mem -> Prop :=
-  <{ * ethernet_header h a
-     * array (uint 8) n bs (a ^+ /[sizeof ethernet_header])
-     * array (uint 8) (MBUF_SIZE - n - sizeof ethernet_header) ?
-         (a ^+ /[sizeof ethernet_header + n]) }>.
- TODO define using mbuf? *)
 
 Definition eth_buff(h: ethernet_header_t)(n: Z)(zs: list Z): word -> mem -> Prop.
 Admitted.
@@ -100,7 +64,7 @@ Definition ethernet_reply(req_h: ethernet_header_t)(resp_payload: word -> mem ->
 Definition IPv4_WITH_NO_OPTIONS := Z.lor (Z.shiftl 4 4) 5.
 Definition IP_TTL := 64.
 
-Definition ip_reply(req_h: headers_upto_ip)(proto: Z)(resp_payload: word -> mem -> Prop)
+Definition ip_reply(req_h: headers_upto_ip_t)(proto: Z)(resp_payload: word -> mem -> Prop)
   {resp_payload_sz: PredicateSize resp_payload}: word -> mem -> Prop :=
   ethernet_reply (before_ip_header req_h)
     <{ + ip_header {|
@@ -122,7 +86,7 @@ Definition IP_PROTO_ICMP := 1.
 Definition IP_PROTO_TCP := 6.
 Definition IP_PROTO_UDP := 17.
 
-Definition udp_reply(req_h: headers_upto_udp)(resp_payload: word -> mem -> Prop)
+Definition udp_reply(req_h: headers_upto_udp_t)(resp_payload: word -> mem -> Prop)
   {resp_payload_sz: PredicateSize resp_payload}: word -> mem -> Prop :=
   ip_reply (before_udp_header req_h) IP_PROTO_UDP
     <{ + udp_header {|
@@ -135,16 +99,20 @@ Definition udp_reply(req_h: headers_upto_udp)(resp_payload: word -> mem -> Prop)
 
 Import ReversedListNotations.
 
+(*
 Instance spec_of_net_tx_udp: fnspec :=                                          .**/
 
 void net_tx_udp(uintptr_t nw, uintptr_t b, uintptr_t n,
                 uintptr_t dst_ip, uintptr_t dstPort, uintptr_t srcPort) /**#
-  ghost_args := bs pks foo req_h (R: mem -> Prop);
-  requires t m := <{ * mbuf.mbuf \[n] bs b (* TODO udp_buf *)
+  ghost_args := (body: word -> mem -> Prop)
+                pks foo req_h (R: mem -> Prop);
+  requires t m := <{ * network nw
+                     * mbuf \[n] (anyval headers_upto_udp) (*<{ + anyval headers_upto_udp
+                                    + body }>*) b
                      * R }> m;
-  ensures t' m' := t' = t /\ foo (pks ;+ TxPacket (udp_reply req_h (array (uint 8) \[n] bs)))
+  ensures t' m' := t' = t /\ foo (pks ;+ TxPacket (udp_reply req_h body))
     /\ <{ * R * R }> m' #**/                                                   /**.
-
+*)
 
 (** * Receive, top-down: *)
 
@@ -156,12 +124,11 @@ Instance spec_of_net_rx_eth: fnspec :=                                          
 
 void net_rx_eth(uintptr_t a, uintptr_t n) /**#
   ghost_args := bs (R: mem -> Prop);
-  requires t m := <{ * mbuf.mbuf \[n] bs a
+  requires t m := <{ * mbuf \[n] bs a
                      * R }> m;
   (* rx may change the mbuf arbitrarily, but must return it *)
   ensures t' m' := t' = t /\ exists bs' n',
-       <{ * mbuf.mbuf n' bs' a
+       <{ * mbuf n' bs' a
           * R }> m' #**/                                                   /**.
-
 
 End LiveVerif. Comments .**/ //.
